theories/helpers.v
@@ -1,4 +1,31 @@
 From stdpp Require Import list.
+From iris.proofmode Require Import proofmode.
+From iris.heap_lang Require Import proofmode notation.
+
+Section heap.
+  Context `{!heapGS Σ} (N : namespace).
+
+  Lemma array_agree x l1 l2 dq1 dq2 :
+    length l1 = length l2 →
+    x ↦∗{dq1} l1 -∗ x ↦∗{dq2} l2 -∗ ⌜l1 = l2⌝.
+  Proof.
+    revert l2.
+    iInduction l1 as [|v l1] "HInd" using rev_ind;
+      iIntros (l2 HL) "x1 x2".
+      { destruct l2; auto. }
+    destruct l2 using rev_ind.
+      { rewrite app_length in HL. simpl in HL. lia. }
+    clear IHl2.
+
+    do 2 rewrite array_app.
+    assert (length l1 = length l2).
+      { do 2 rewrite app_length in HL. simpl in HL. lia. }
+    iDestruct "x1" as "[x1 xl1]". iDestruct "x2" as "[x2 xl2]".
+    do 2 rewrite array_singleton. rewrite H.
+    iDestruct (mapsto_agree with "xl1 xl2") as "<-".
+    iDestruct ("HInd" $! l2 with "[] [x1] [x2]") as "<-"; auto.
+  Qed.
+End heap.
 
 Section slice.
   Context {A : Type}.
@@ -9,4 +36,22 @@ Section slice.
 
   Lemma slice_0 l i : slice l i 0 = [].
   Proof. auto. Qed.
+
+  Lemma slice_insert_right l i k j v :
+    j >= i + k →
+    slice (<[j:=v]> l) i k = slice l i k.
+  Proof.
+    unfold slice. intros H.
+    rewrite drop_insert_le; [|lia].
+    rewrite take_insert; auto. lia.
+  Qed.
+
+  Lemma slice_extend_right l i k v :
+    l !! (i+k) = Some v →
+    slice l i (S k) = slice l i k ++ [v].
+  Proof.
+    unfold slice. intros H.
+    rewrite (take_S_r _ _ v); auto.
+    by rewrite lookup_drop.
+  Qed.
 End slice.
